IMLTT/proofs/admissable/Lifting.lean
@@ -1,0 +1,6 @@
+import IMLTT.AbstractSyntax
+import IMLTT.Substitution
+import IMLTT.JudgmentsAndRules
+
+theorem lifting_ctx_one_term : Γ ⬝ (lift i j A) = Γ, (lift_ctx i j (Ctx.empty ⬝ A)) :=
+  sorry
