IMLTT/proofs/admissable/Weakening.lean
@@ -1,6 +1,30 @@
+import IMLTT.AbstractSyntax
+import IMLTT.Substitution
+import IMLTT.JudgmentsAndRules
 
 /- # Weakening -/
 
--- TODO: formulate theorems for all forms of judgment
--- TODO: substitution property in Harpter and Pfenning
+theorem weakening_ctx : IsCtx (Γ ⬝ A) → IsType Γ B
+                        → IsCtx (Γ ⬝ B ⬝ (lift 0 1 A)) :=
+  by
+    sorry
 
+theorem weakening_type : IsType Γ A → IsType Γ B
+                         → IsType (Γ ⬝ B) (lift 0 1 A) :=
+  by
+    sorry
+
+theorem weakening_term : HasType Γ a A → IsType Γ B
+                         → HasType (Γ ⬝ B) (lift 0 1 a) (lift 0 1 A) :=
+  by
+    sorry
+
+theorem weakening_type_eq : IsEqualType (Γ, Δ) A A' → IsType Γ B
+                            → IsEqualType (Γ ⬝ B, (lift_ctx 0 1 Δ)) (lift 0 1 A) (lift 0 1 A') :=
+  by
+    sorry
+
+theorem weakening_term_eq : IsEqualTerm Γ a a' A → IsType Γ B
+                            → IsEqualTerm (Γ ⬝ B) (lift 0 1 a) (lift 0 1 a') (lift 0 1 A') :=
+  by
+    sorry 
